@prefix dc: <http://purl.org/dc/elements/1.1/> .
@prefix dct: <http://purl.org/dc/terms/> .
@prefix mbs: <https://w3id.org/mibact-sapienza/> .
@prefix rdf: <http://www.w3.org/1999/02/22-rdf-syntax-ns#> .
@prefix skos: <http://www.w3.org/2004/02/skos/core#> .

<https://w3id.org/mibact-sapienza/> a skos:ConceptScheme;
  dc:creator "Sapienza University of Rome"@en;
  dct:description "Vocabulary compiled for the LCD2 pilot"@en;
  dct:rights <https://creativecommons.org/licenses/by/4.0/>;
  dct:title "Risk Map vocabulary"@en;
  skos:hasTopConcept mbs:1, mbs:10, mbs:11, mbs:8, mbs:9 .

mbs:1 a skos:Concept;
  skos:inScheme <https://w3id.org/mibact-sapienza/>;
  skos:narrower mbs:2, mbs:3, mbs:4, mbs:5;
  skos:prefLabel "centro storico"@it, "historical centre"@en;
  skos:scopeNote "Ensemble of historic buildings within an urban agglomeration formed by World War I (1919).This chronological threshold normally identifies a part - generally central - of the town, but the contemporary city can also include several historical districts that are in fact disjointed. This center is delimited by a perimetration that can sometimes coincide with the boundary of the walls when it still exists or when it can be identified on the basis of historical cadastres or the material evidence of the building, or with some natural limits (streams, strong slopes, etc.) sometimes it results from the evident constructive mutation of the building, verified by the comparison with the available cartographic and historical graphic docuemnation and direct feedback."@en;
  skos:topConceptOf <https://w3id.org/mibact-sapienza/> .

mbs:2 a skos:Concept;
  skos:broader mbs:1;
  skos:inScheme <https://w3id.org/mibact-sapienza/>;
  skos:prefLabel "spazio urbano"@it, "urban space"@en;
  skos:related mbs:11, mbs:7;
  skos:scopeNote "it constitutes an open space inside the historic center bordered by several 'urban fronts' and characterized by the presence of specific elements (gardens, furnishings, flooring, etc.). In theory, all the streets, squares and wide slars contained within the center are urban spaces."@en .

mbs:3 a skos:Concept;
  skos:broader mbs:1;
  skos:inScheme <https://w3id.org/mibact-sapienza/>;
  skos:narrower mbs:6;
  skos:prefLabel "unità urbana"@it, "urban unit"@en;
  skos:related mbs:5;
  skos:scopeNote "It constitutes a portion of the built fabric of the historic center morphologically and structurally autonomous and clearly identifiable. It appears to be bounded by a variable number of fronts, all or part of which are on urban spaces with whom it communicates through the access to the ground floor. The urban unit can be constituted as an 'aggregate' or as a 'residential or specialistic punctual building unit'"@en .

mbs:4 a skos:Concept;
  skos:broader mbs:1;
  skos:inScheme <https://w3id.org/mibact-sapienza/>;
  skos:prefLabel "Unità urbana-aggregato"@it, "urban units-aggregates"@en;
  skos:related mbs:2;
  skos:scopeNote "It is a type of 'urban unit' and is understood as a continuous set of structurally connected but distinguishable building units as organisms that are architecturally coherent. It is bordered by urban spaces with which it communicates through accesses to the ground floor and may contain within it places relevant to one or more building units. It overlooks on urban spaces through fronts that result from the succession of the individual facades of the building units."@en .

mbs:5 a skos:Concept;
  skos:broader mbs:1;
  skos:inScheme <https://w3id.org/mibact-sapienza/>;
  skos:prefLabel "unità urbana-edilizia puntuale residenziale o specialistica"@it, "urban units-residential or specialistic punctual buildings"@en;
  skos:related mbs:2, mbs:3;
  skos:scopeNote "It is a type of 'urban unit' and is understood as a homogeneous and autonomous unitary element. It is bordered by urban spaces with whom it communicates through accesses to the ground floor and can contain open places inside. It overlooks urban spaces through a variable number of fronts generally figuratively and constructively coherent with each other. 'Residential punctual building units' are buildings such as villas or cottages, while 'Specialist punctual building units' include hospitals or schools."@en .

mbs:6 a skos:Concept;
  skos:broader mbs:3;
  skos:inScheme <https://w3id.org/mibact-sapienza/>;
  skos:narrower mbs:7;
  skos:prefLabel "building unit"@en, "unità edilizia"@it;
  skos:scopeNote "It is a coherent architectural organism, consisting in a single construction phase or by the merging/recasting of several pre-existing building units. This organism is characterized by the presence of one or more functional units (residential and non-residential) connected to each other through common distribution elements and served by access at the road level; it is bordered by external facades with a generally continuous eaves line and a unitary or composite roof composed of flat and/or inclined parts consistent with all fronts."@en .

mbs:7 a skos:Concept;
  skos:broader mbs:6;
  skos:inScheme <https://w3id.org/mibact-sapienza/>;
  skos:prefLabel "building front"@en, "fronte edilizio"@it;
  skos:related mbs:2;
  skos:scopeNote "It corresponds to the façade of the single 'building unit' overlooking on an urban space or, more generally, on a street or a town square but also on the natural margin of the town (maritime, river, lake coast, prmonatory limit, etc.)."@en .

mbs:8 a skos:Concept;
  skos:inScheme <https://w3id.org/mibact-sapienza/>;
  skos:prefLabel "architectural heritage"@en, "bene architettonico"@it;
  skos:related mbs:1;
  skos:scopeNote "Built works transmitted inter-generationally within a society and that are invested with significance in that society (AAT scope note)"@en;
  skos:topConceptOf <https://w3id.org/mibact-sapienza/> .

mbs:9 a skos:Concept;
  skos:inScheme <https://w3id.org/mibact-sapienza/>;
  skos:prefLabel "archeological heritage"@en, "bene archeologico"@it;
  skos:related mbs:1;
  skos:scopeNote "Built works remains of past human life and activities, generally referred to a period ranging from ancient to early medieval time."@en;
  skos:topConceptOf <https://w3id.org/mibact-sapienza/> .

mbs:10 a skos:Concept;
  skos:inScheme <https://w3id.org/mibact-sapienza/>;
  skos:prefLabel "parchi"@it, "parks"@en;
  skos:related mbs:1;
  skos:scopeNote "Permanently dedicated recreation areas, often open to the public and generally characterized by their natural, historic, or landscape features; often administered by governmental agencies (AAT scope note)."@en;
  skos:topConceptOf <https://w3id.org/mibact-sapienza/> .

mbs:11 a skos:Concept;
  skos:inScheme <https://w3id.org/mibact-sapienza/>;
  skos:prefLabel "gardens"@en, "giardini"@it;
  skos:related mbs:1, mbs:2;
  skos:scopeNote "Area of ground or open space; usually, but not always, where flowers, shrubs, trees, vegetables, or fruits are grown and cultivated (AAT scope note)."@en;
  skos:topConceptOf <https://w3id.org/mibact-sapienza/> .
